Fix weird mess

theories/OGS/Soundness.v
@@ -1,1 +1,60 @@
-capybara@Capybara.local.36540
+From Coinduction Require Import coinduction tactics.
+
+From OGS Require Import Prelude.
+From OGS.Utils Require Import Ctx Rel.
+From OGS.Game Require Import HalfGame Event.
+From OGS.OGS Require Import Subst Obs Machine Game Strategy Utility_lemmas CompGuarded Adequacy Congruence.
+From OGS.ITree Require Import ITree Eq Delay Structure Properties Guarded.
+
+Open Scope ctx_scope.
+
+Section withFam.
+
+(*|
+We consider a language abstractly captured as a machine
+|*)
+  Context {bT : baseT}.
+  Context {bV : baseV}.
+  Context {bC : baseC}.
+  Context {sV : subst_monoid bV}.
+  Context {sC : subst_module bV bC}.
+  Context {oS : observation_structure}.
+  Context {M: machine}.
+(*|
+Satisfying an appropriate axiomatization
+|*)
+  Context {sVL: subst_monoid_laws}.
+  Context {sCL: subst_module_laws}.
+  Context {VA : var_assumptions} .
+  Context {ML: machine_laws}.
+
+  Definition ciu {Γ} Δ (x y : conf Γ) : Prop
+    := forall e : Γ ⇒ᵥ Δ, eval_in_env e x ≈ eval_in_env e y.
+  Notation "x ≈⟦ciu Δ ⟧≈ y" := (ciu Δ x y) (at level 50).
+
+  Definition barb {Γ} Δ (x y : conf Γ) : Prop
+    := forall e : Γ ⇒ᵥ Δ, (inj_init_act Δ x ∥ inj_init_pas e) ≈ (inj_init_act Δ y ∥ inj_init_pas e).
+  Notation "x ≈⟦barb Δ ⟧≈ y" := (barb Δ x y) (at level 50).
+
+  Theorem barb_correction {Γ} Δ (x y : conf Γ) : x ≈⟦barb Δ ⟧≈ y -> x ≈⟦ciu Δ ⟧≈ y.
+  Proof.
+    intros H e.
+    etransitivity; [ apply it_eq_wbisim, (adequacy x e) | ].
+    etransitivity; [ apply iter_evg_iter | ].
+    etransitivity; [ apply (H e) | symmetry ].
+    etransitivity; [ apply it_eq_wbisim, (adequacy y e) | ].
+    etransitivity; [ apply iter_evg_iter | ].
+    reflexivity.
+  Qed.
+
+  Theorem ogs_correction {Γ} Δ (x y : conf Γ) : x ≈⟦ogs Δ ⟧≈ y -> x ≈⟦ciu Δ ⟧≈ y.
+  Proof.
+    intro H; apply barb_correction.
+    intro e; unfold compo.
+    rewrite <- 2 compo_compo_alt.
+    apply compo_alt_proper; [ exact H | intro; reflexivity ].
+  Qed.
+
+End withFam.
+About ogs_correction.
+Print Assumptions ogs_correction.
